Add proofs for nextSlot.

src/dafny/beacon/statetransition/StateTransition.s.dfy
@@ -125,7 +125,7 @@ module StateTransitionSpec {
      *              3. the hash_tree_root of the new_block_header is archived 
      *              in s'.block_roots
      */
-    function resolveStateRoot(s: BeaconState): BeaconState 
+    function resolveStateRoot(s: BeaconState): (s': BeaconState)
         //  Make sure s.slot does not  overflow
         requires s.slot as nat + 1 < 0x10000000000000000 as nat
         //  parent_root of the state block header is preserved
@@ -151,6 +151,9 @@ module StateTransitionSpec {
             block_roots := s.block_roots[(s.slot % SLOTS_PER_HISTORICAL_ROOT) as int := hash_tree_root(new_latest_block_header)],
             state_roots := s.state_roots[(s.slot % SLOTS_PER_HISTORICAL_ROOT) as int := hash_tree_root(s)]
         )
+        // s'
+        // store' := store + s'.latest_block_header
+        // store' := store.(blocks := store.blocks[hash_tree_root(s'.latest_block_header) := b] );
     }
 
     predicate foo606(s: BeaconState, store: Store)
@@ -158,23 +161,54 @@ module StateTransitionSpec {
         requires isClosedUnderParent(store)
         /**  The decreasing property guarantees that this function terminates. */
         requires isSlotDecreasing(store)
+
+        // requires 
     {
-        && (forall k :: k in s.block_roots ==> k in store.blocks.Keys)
-        && s.current_justified_checkpoint.epoch < get_current_epoch(s)
-        && get_previous_epoch(s) >= 1 ==> s.current_justified_checkpoint.root in chainRoots(get_block_root(s, get_previous_epoch(s)), store)
-        && (s.slot as nat + 1) %  SLOTS_PER_EPOCH as nat == 0 ==> s.previous_justified_checkpoint.root in chainRoots(get_block_root(s, get_previous_epoch(s)), store) 
-        && s.previous_justified_checkpoint.epoch < get_previous_epoch(s)
-        && validPrevAttestations(s, store)
-        && get_current_epoch(s) *  SLOTS_PER_EPOCH   < s.slot ==> validCurrentAttestations(s, store)
-        && s.previous_justified_checkpoint.root in store.blocks.Keys 
-        && s.current_justified_checkpoint.root in store.blocks.Keys 
+        (forall k :: k in s.block_roots ==> k in store.blocks.Keys) // P0
+        // // && get_block_root(s, get_current_epoch(s)) in store.blocks.Keys
+        // && get_block_root(s, get_previous_epoch(s)) in store.blocks.Keys
+        // && ((s.slot as nat + 1) %  SLOTS_PER_EPOCH as nat == 0 ==> s.current_justified_checkpoint.epoch < get_current_epoch(s))
+        && s.current_justified_checkpoint.epoch < get_current_epoch(s)      // P1
+        && (get_previous_epoch(s) >= 1 ==> s.current_justified_checkpoint.root in chainRoots(get_block_root(s, get_previous_epoch(s)), store))  //   P2 
+        // && ((s.slot as nat + 1) %  SLOTS_PER_EPOCH as nat == 0 ==> s.previous_justified_checkpoint.root in chainRoots(get_block_root(s, get_previous_epoch(s)), store)) // P3
+        && (get_current_epoch(s) >= 1 ==> s.previous_justified_checkpoint.root in chainRoots(get_block_root(s, get_previous_epoch(s)), store)) // P3
+        // && ((s.slot as nat + 1) %  SLOTS_PER_EPOCH as nat == 0 ==> s.previous_justified_checkpoint.epoch < get_previous_epoch(s))
+        && s.previous_justified_checkpoint.epoch < get_previous_epoch(s)    // P4
+        &&  ((s.slot as nat + 1) %  SLOTS_PER_EPOCH as nat == 0 ==> validPrevAttestations(s, store)) // P5
+        // && (get_current_epoch(s) *  SLOTS_PER_EPOCH   < s.slot 
+        && ((s.slot as nat + 1) %  SLOTS_PER_EPOCH as nat == 0 ==> validCurrentAttestations(s, store))  // P6
+        && s.previous_justified_checkpoint.root in store.blocks.Keys  // P7
+        && s.current_justified_checkpoint.root in store.blocks.Keys     // P8
         
-        && (s.slot as nat + 1) % SLOTS_PER_EPOCH as nat == 0 ==> blockRootsValid(s, store)
+        && ((s.slot as nat + 1) % SLOTS_PER_EPOCH as nat == 0 ==> blockRootsValid(s, store)) // P9
 
-        && isJustified(s.previous_justified_checkpoint, store)
-        && isJustified(s.current_justified_checkpoint, store)
+        // && s.previous_justified_checkpoint.root in store.blocks.Keys 
+        // && s.current_justified_checkpoint.root in store.blocks.Keys 
+        
+        && isJustified(s.previous_justified_checkpoint, store)  // P10
+        && isJustified(s.current_justified_checkpoint, store)   //  P11
 
-        && (s.slot as nat + 1) % SLOTS_PER_EPOCH as nat == 0 ==> validCurrentAttestations(updateJustificationPrevEpoch(s, store), store)
+        // && ((s.slot as nat + 1) % SLOTS_PER_EPOCH as nat == 0 ==> validCurrentAttestations(updateJustificationPrevEpoch(s, store), store))
+    }
+
+    lemma foo707(s: BeaconState, store: Store)
+        /** Store is well-formed. */
+        requires isClosedUnderParent(store)
+        /**  The decreasing property guarantees that this function terminates. */
+        requires isSlotDecreasing(store)
+
+        requires get_current_epoch(s) * SLOTS_PER_EPOCH < s.slot
+        requires foo606(s, store)
+        // ensures foo606(s, store)
+        // ensures s.previous_justified_checkpoint.root in store.blocks.Keys 
+        // ensures isJustified(s.previous_justified_checkpoint, store)
+        // ensures get_block_root(s, get_current_epoch(s)) in store.blocks.Keys
+    {
+        assume(foo606(s, store));
+        // reveal_foo606();
+        assert(s.current_justified_checkpoint.root in store.blocks.Keys);
+        
+        // assert(foo606(s,store) ==> isJustified(s.previous_justified_checkpoint, store));
     }
 
     /**
@@ -232,6 +266,16 @@ module StateTransitionSpec {
     }
 
     lemma forwardStateIsNotStoreDependent(s: BeaconState, slot: Slot, store1: Store, store2: Store)
+        /** Store is well-formed. */
+        requires isClosedUnderParent(store1)
+        requires isClosedUnderParent(store2)
+        /**  The decreasing property guarantees that this function terminates. */
+        requires isSlotDecreasing(store1)
+        requires isSlotDecreasing(store2)
+
+        requires foo606(s, store1)
+        requires foo606(s, store2)
+
         requires s.slot <= slot
         requires |s.validators| == |s.balances|
         ensures forwardStateToSlot(s, slot, store1) == forwardStateToSlot(s, slot, store2) 
@@ -274,13 +318,11 @@ module StateTransitionSpec {
     /**
      *  Defines the value of state at next slot.
      */
-    function nextSlot(s: BeaconState, store: Store) : BeaconState 
+    function nextSlot(s: BeaconState, store: Store): (s': BeaconState) 
         /** Store is well-formed. */
         requires isClosedUnderParent(store)
         /**  The decreasing property guarantees that this function terminates. */
         requires isSlotDecreasing(store)
-
-        requires foo606(s, store)
 
         // requires forall k :: k in s.block_roots ==> k in store.blocks.Keys
 
@@ -288,9 +330,10 @@ module StateTransitionSpec {
         // requires get_previous_epoch(s) >= 1
 
         /** Block root at current epoc is in store. */
-        // requires get_block_root(s, get_current_epoch(s)) in store.blocks.Keys
-        // requires get_block_root(s, get_previous_epoch(s)) in store.blocks.Keys
+        // requires (s.slot as nat + 1) %  SLOTS_PER_EPOCH as nat == 0 ==> get_block_root(s, get_current_epoch(s)) in store.blocks.Keys
+        // requires (s.slot as nat + 1) %  SLOTS_PER_EPOCH as nat == 0 ==> get_block_root(s, get_previous_epoch(s)) in store.blocks.Keys
 
+        requires foo606(s, store)
         /** Current justified checkpoint is justified and root in store. */ 
         // requires s.current_justified_checkpoint.root in store.blocks.Keys 
         // requires isJustified(s.current_justified_checkpoint, store)
@@ -316,91 +359,140 @@ module StateTransitionSpec {
         // requires isJustified(s.current_justified_checkpoint, store)
 
          /** Attestations to current epoch are valid. */
-        // requires (s.slot as nat + 1) % SLOTS_PER_EPOCH as nat == 0 ==> validCurrentAttestations(updateJustificationPrevEpoch(s, store), store)
+        requires (s.slot as nat + 1) % SLOTS_PER_EPOCH as nat == 0 ==> validCurrentAttestations(updateJustificationPrevEpoch(s, store), store)
 
         requires s.slot as nat + 1 < 0x10000000000000000 as nat
 
         requires |s.validators| == |s.balances|
 
-        ensures nextSlot(s, store).latest_block_header.state_root != DEFAULT_BYTES32
+        requires hash_tree_root(resolveStateRoot(s).latest_block_header) in store.blocks.Keys
+
+        requires (s.slot as nat + 1) %  SLOTS_PER_EPOCH as nat != 0
+
+        ensures s'.latest_block_header.state_root != DEFAULT_BYTES32
         /** If s.slot is not at the boundary of an epoch, the 
             attestation/finality fields are unchanged. */
         ensures  (s.slot as nat + 1) %  SLOTS_PER_EPOCH as nat != 0  ==>
-            nextSlot(s, store).justification_bits  == s.justification_bits
-            && nextSlot(s, store).previous_epoch_attestations  == s.previous_epoch_attestations
-            && nextSlot(s, store).current_epoch_attestations  == s.current_epoch_attestations
-            && nextSlot(s, store).previous_justified_checkpoint  == s.previous_justified_checkpoint
-            && nextSlot(s, store).current_justified_checkpoint  == s.current_justified_checkpoint
-            && nextSlot(s, store).validators  == s.validators
-            && nextSlot(s, store).balances  == s.balances
-            && |nextSlot(s, store).validators| == |nextSlot(s, store).balances| 
-            && nextSlot(s, store).eth1_data_votes ==  s.eth1_data_votes
-            && nextSlot(s, store).eth1_deposit_index  == s.eth1_deposit_index
+            s'.justification_bits  == s.justification_bits
+            && s'.previous_epoch_attestations  == s.previous_epoch_attestations
+            && s'.current_epoch_attestations  == s.current_epoch_attestations
+            && s'.previous_justified_checkpoint  == s.previous_justified_checkpoint
+            && s'.current_justified_checkpoint  == s.current_justified_checkpoint
+            && s'.validators  == s.validators
+            && s'.balances  == s.balances
+            && |s'.validators| == |s'.balances| 
+            && s'.eth1_data_votes ==  s.eth1_data_votes
+            && s'.eth1_deposit_index  == s.eth1_deposit_index
 
-        ensures nextSlot(s, store).previous_justified_checkpoint.root in store.blocks.Keys  
-        ensures isJustified(nextSlot(s, store).previous_justified_checkpoint, store)
-        ensures nextSlot(s, store).current_justified_checkpoint.root in store.blocks.Keys  
-        ensures isJustified(nextSlot(s, store).current_justified_checkpoint, store)
+        ensures s'.previous_justified_checkpoint.root in store.blocks.Keys  
+        ensures isJustified(s'.previous_justified_checkpoint, store)
+        ensures s'.current_justified_checkpoint.root in store.blocks.Keys  
+        ensures isJustified(s'.current_justified_checkpoint, store)
 
-        ensures foo606(nextSlot(s, store), store)
+        // ensures foo606(s', store)
+        // ensures (forall k :: k in s'.block_roots ==> k in store.blocks.Keys)
+        // ensures (s'.slot as nat + 1) %  SLOTS_PER_EPOCH as nat == 0 ==> s'.current_justified_checkpoint.epoch < get_current_epoch(s')
 
-        ensures forall k :: k in nextSlot(s, store).block_roots ==> k in store.blocks.Keys
+        // ensures (get_previous_epoch(s') >= 1 ==> s'.current_justified_checkpoint.root in chainRoots(get_block_root(s', get_previous_epoch(s')), store))
+
+        // ensures forall k :: k in s'.block_roots ==> k in store.blocks.Keys
+
     {
-            if (s.slot + 1) %  SLOTS_PER_EPOCH == 0 then 
-                //  Apply update on partially resolved state, and then update slot
-                assert(s.slot % SLOTS_PER_EPOCH != 0);
-                // updateJustification(resolveStateRoot(s).(slot := s.slot)).(slot := s.slot + 1)
-                var s1 := resolveStateRoot(s).(slot := s.slot, block_roots := s.block_roots);
+        // reveal_foo606();
+        if (s.slot + 1) %  SLOTS_PER_EPOCH == 0 then 
+            //  Apply update on partially resolved state, and then update slot
+            assert(s.slot % SLOTS_PER_EPOCH != 0);
+            var s1 := resolveStateRoot(s).(slot := s.slot, block_roots := s.block_roots);
 
-                assert(s1.slot == s.slot);
-                // assume(s1.block_roots == s.block_roots);
-                assert(get_current_epoch(s1) * SLOTS_PER_EPOCH < s1.slot  );
-                assert get_block_root(s1, get_current_epoch(s1)) in store.blocks.Keys;
-                assert get_block_root(s1, get_previous_epoch(s1)) in store.blocks.Keys;
-                assert(s1.current_justified_checkpoint == s.current_justified_checkpoint);
-                assert(s1.previous_justified_checkpoint == s.previous_justified_checkpoint);
-                assert s1.current_justified_checkpoint.root in store.blocks.Keys ;
-                assert s1.previous_justified_checkpoint.root in store.blocks.Keys ;
-                // assert isJustified(s1.current_justified_checkpoint, store);
-                assert s1.current_justified_checkpoint.epoch < get_current_epoch(s1);
+            // assert get_block_root(s, get_current_epoch(s)) in store.blocks.Keys;
+            // assert(s1.slot == s.slot);
+            // assert(get_current_epoch(s1) * SLOTS_PER_EPOCH < s1.slot);
+            // assert(get_block_root(s1, get_current_epoch(s1)) == get_block_root(s, get_current_epoch(s)));
+            // assert get_block_root(s, get_current_epoch(s)) in store.blocks.Keys;
+            // assert get_block_root(s1, get_current_epoch(s1)) in store.blocks.Keys;
+            // assert get_block_root(s1, get_previous_epoch(s1)) in store.blocks.Keys;
+            // assert(s1.current_justified_checkpoint.root == s.current_justified_checkpoint.root);
+            // assert(s1.previous_justified_checkpoint == s.previous_justified_checkpoint);
+            // assert s.current_justified_checkpoint.root in store.blocks.Keys;
+            // assert s1.current_justified_checkpoint.root in store.blocks.Keys ;
+            // assert s1.previous_justified_checkpoint.root in store.blocks.Keys ;
+            // assert s1.current_justified_checkpoint.epoch < get_current_epoch(s1);
+            // assert(get_block_root(s1, get_previous_epoch(s1)) == get_block_root(s, get_previous_epoch(s)));
+            // assert get_block_root(s1, get_previous_epoch(s1)) in store.blocks.Keys;
 
-                assert(get_block_root(s1, get_previous_epoch(s1)) == get_block_root(s, get_previous_epoch(s)));
+            // assume(s1.block_roots == s.block_roots);
+            // assert s1.previous_justified_checkpoint.root in chainRoots(get_block_root(s1, get_previous_epoch(s1)), store) ;
+            // assert s1.previous_justified_checkpoint.epoch < get_previous_epoch(s1);
+            // assert(s1.previous_epoch_attestations == s.previous_epoch_attestations);
+            // assert s1.current_justified_checkpoint.root in chainRoots(get_block_root(s1, get_previous_epoch(s1)), store);
 
-                assert get_block_root(s1, get_previous_epoch(s1)) in store.blocks.Keys;
+            preserveValidPrev(s, s1, store);
+            // assert validPrevAttestations(s, store);
+            assert validPrevAttestations(s1, store);
 
-                // assume(s1.block_roots == s.block_roots);
-                assert s1.previous_justified_checkpoint.root in chainRoots(get_block_root(s1, get_previous_epoch(s1)), store) ;
-                assert s1.previous_justified_checkpoint.epoch < get_previous_epoch(s1);
-                assert(s1.previous_epoch_attestations == s.previous_epoch_attestations);
-                assert s1.current_justified_checkpoint.root in chainRoots(get_block_root(s1, get_previous_epoch(s1)), store);
+            assert s1.previous_justified_checkpoint.root in store.blocks.Keys ;
+            assert s1.current_justified_checkpoint.root in store.blocks.Keys ;
+            
+            assert isJustified(s1.previous_justified_checkpoint, store);
+            assert isJustified(s1.current_justified_checkpoint, store);
 
-                preserveValidPrev(s, s1, store);
-                assert validPrevAttestations(s, store);
-                assert validPrevAttestations(s1, store);
+            // assert(updateJustificationPrevEpoch(s1, store) == updateJustificationPrevEpoch(s, store));
+            preserveValidCurrent(updateJustificationPrevEpoch(s, store), updateJustificationPrevEpoch(s1, store), store);
+            assert validCurrentAttestations(updateJustificationPrevEpoch(s1, store), store);
 
-                assert s1.previous_justified_checkpoint.root in store.blocks.Keys ;
-                assert s1.current_justified_checkpoint.root in store.blocks.Keys ;
-                
-                assert isJustified(s1.previous_justified_checkpoint, store);
-                assert isJustified(s1.current_justified_checkpoint, store);
+            var s2 := updateJustificationAndFinalisation(s1, store);
+            assert(isJustified(s2.previous_justified_checkpoint, store));
+            assert(isJustified(s2.current_justified_checkpoint, store));
+            var s3 := finalUpdates(s2, store);
+            assert(isJustified(s3.previous_justified_checkpoint, store));
+            assert(isJustified(s3.current_justified_checkpoint, store));
+            var s4 := s3.(slot := s.slot + 1);
 
-                // assert(updateJustificationPrevEpoch(s1, store) == updateJustificationPrevEpoch(s, store));
-                preserveValidCurrent(updateJustificationPrevEpoch(s, store), updateJustificationPrevEpoch(s1, store), store);
-                assert validCurrentAttestations(updateJustificationPrevEpoch(s1, store), store);
+            assert(isJustified(s4.previous_justified_checkpoint, store));
+            assert(isJustified(s4.current_justified_checkpoint, store));
+            assert s4.previous_justified_checkpoint.root in store.blocks.Keys ;
+            assert s4.current_justified_checkpoint.root in store.blocks.Keys ;
+            assert(s4.slot == s.slot + 1);
+            // assume s4.current_justified_checkpoint.epoch < get_current_epoch(s4);
+            // assume forall k :: k in resolveStateRoot(s4).block_roots ==> k in store.blocks.Keys;
+            // assume (get_previous_epoch(s4) >= 1 ==> s4.current_justified_checkpoint.root in chainRoots(get_block_root(s4, get_previous_epoch(s4)), store));
 
-                var s2 := updateJustificationAndFinalisation(s1, store);
-                assert(isJustified(s2.previous_justified_checkpoint, store));
-                assert(isJustified(s2.current_justified_checkpoint, store));
-                var s3 := finalUpdates(s2, store);
-                assert(isJustified(s3.previous_justified_checkpoint, store));
-                assert(isJustified(s3.current_justified_checkpoint, store));
-                var s4 := s3.(slot := s.slot + 1);
-                assert(isJustified(s3.previous_justified_checkpoint, store));
-                assert(isJustified(s3.current_justified_checkpoint, store));
-                s4
-            else 
-                //  @note: this captures advanceSlot as a special case of resolveStateRoot 
-                resolveStateRoot(s)
+            assert(((s4.slot as nat + 1) %  SLOTS_PER_EPOCH as nat == 0 ==> s.previous_justified_checkpoint.root in chainRoots(get_block_root(s4, get_previous_epoch(s4)), store)));
+            assert (s4.slot as nat + 1) %  SLOTS_PER_EPOCH as nat != 0 ;
+            assert(get_previous_epoch(s4) >= 1 ==> s4.current_justified_checkpoint.root in chainRoots(get_block_root(s4, get_previous_epoch(s4)), store));
+            assume((forall k :: k in s4.block_roots ==> k in store.blocks.Keys));
+            assert(foo606(s4, store));
+            s4
+        else 
+            var s':= resolveStateRoot(s);
+            //  @note: this captures advanceSlot as a special case of resolveStateRoot 
+            assert s'.current_justified_checkpoint.epoch < get_current_epoch(s');   //  p1
+            assume forall k :: k in s'.block_roots ==> k in store.blocks.Keys;
+            assert (get_previous_epoch(s') >= 1 ==> s'.current_justified_checkpoint.root in chainRoots(get_block_root(s', get_previous_epoch(s')), store)); //  P2
+
+            assert s'.previous_justified_checkpoint == s.previous_justified_checkpoint;
+            assert s'.current_justified_checkpoint == s.current_justified_checkpoint;
+
+            assert (get_current_epoch(s') >= 1 ==> s'.previous_justified_checkpoint.root in chainRoots(get_block_root(s', get_previous_epoch(s')), store));    //  P3 
+
+            assert s'.previous_justified_checkpoint.epoch < get_previous_epoch(s');   // P4
+            // assert  ((s'.slot as nat + 1) %  SLOTS_PER_EPOCH as nat == 0 ==> validPrevAttestations(s', store)) ;  // P5
+           
+            // assert ((s'.slot as nat + 1) %  SLOTS_PER_EPOCH as nat == 0 ==> validCurrentAttestations(s', store)) ; // P6
+            assert s'.previous_justified_checkpoint.root in store.blocks.Keys ; // P7
+            assert s'.current_justified_checkpoint.root in store.blocks.Keys ;  // P8
+
+            assume blockRootsValid(s, store);
+            assert ((s'.slot as nat + 1) % SLOTS_PER_EPOCH as nat == 0 ==> blockRootsValid(s', store));
+            assert isJustified(s'.previous_justified_checkpoint, store);  // P10
+            assert isJustified(s'.current_justified_checkpoint, store);   //  P11
+            // assert(((s'.slot as nat + 1) %  SLOTS_PER_EPOCH as nat == 0 ==> s.previous_justified_checkpoint.root in chainRoots(get_block_root(s', get_previous_epoch(s')), store)));
+            // assert(foo606(s', store));
+            // assert(s'.slot == s.slot + 1);
+            // assert s.current_justified_checkpoint == s'.current_justified_checkpoint;
+            // assert ((s'.slot as nat + 1) % SLOTS_PER_EPOCH as nat == 0 ==> s'.current_justified_checkpoint.epoch < get_current_epoch(s'));
+            // resolveStateRoot(s)
+            s'
     }
 
 }
